compiler/backend/proofs/data_to_word_assignProofScript.sml
@@ -6923,8 +6923,7 @@ Proof
                      wordSemTheory.get_var_imm_def]
   \\ fs [word_cmp_Test_1,word_bit_or,word_bit_if_1_0]
   \\ IF_CASES_TAC THEN1
-   (fs [adj_stk_bignum_def]
-    \\ fs [list_Seq_def,state_rel_thm] \\ eval_tac
+   (fs [list_Seq_def,state_rel_thm] \\ eval_tac
     \\ fs [wordSemTheory.get_vars_def,wordSemTheory.get_var_def,lookup_insert,
            wordSemTheory.set_vars_def,wordSemTheory.set_var_def,alist_insert_def]
     \\ conj_tac THEN1 rw []
@@ -6962,7 +6961,7 @@ Proof
       CCONTR_TAC >> fs[] >>
       qpat_x_assum `w2i _ ≠ _` mp_tac >>
       fs[small_enough_int_w2i_Smallnum_add])
-  \\ fs [adj_stk_bignum_def,stack_consumed_def,OPTION_MAP2_NONE,libTheory.the_def]
+  \\ fs [stack_consumed_def,OPTION_MAP2_NONE,libTheory.the_def]
   \\ unabbrev_all_tac
   \\ rewrite_tac [GSYM state_rel_upd_safe_pkheap]
   \\ match_mp_tac eval_Call_Add
@@ -7030,8 +7029,7 @@ Proof
                      wordSemTheory.get_var_imm_def]
   \\ fs [word_cmp_Test_1,word_bit_or,word_bit_if_1_0]
   \\ IF_CASES_TAC THEN1
-   (fs [adj_stk_bignum_def]
-    \\ fs [list_Seq_def,state_rel_thm] \\ eval_tac
+   (fs [list_Seq_def,state_rel_thm] \\ eval_tac
     \\ fs [wordSemTheory.get_vars_def,wordSemTheory.get_var_def,lookup_insert,
            wordSemTheory.set_vars_def,wordSemTheory.set_var_def,alist_insert_def]
     \\ conj_tac THEN1 rw []
@@ -7070,7 +7068,7 @@ Proof
      ASM_REWRITE_TAC [] >>
      pop_assum kall_tac >>
      fs [small_enough_int_w2i_Smallnum_sub])
-  \\ fs [adj_stk_bignum_def,stack_consumed_def,OPTION_MAP2_NONE,libTheory.the_def]
+  \\ fs [stack_consumed_def,OPTION_MAP2_NONE,libTheory.the_def]
   \\ unabbrev_all_tac
   \\ rewrite_tac [GSYM state_rel_upd_safe_pkheap]
   \\ match_mp_tac eval_Call_Sub
@@ -7103,7 +7101,6 @@ Proof
   match_mp_tac bitTheory.LESS_MULT_MONO2 >>
   strip_tac >> MATCH_ACCEPT_TAC w2n_lt
 QED
-
 
 
 Theorem assign_Mult:
@@ -7149,9 +7146,8 @@ Proof
   \\ fs [wordSemTheory.get_var_def,wordSemTheory.get_var_imm_def,lookup_insert,
          asmTheory.word_cmp_def]
   \\ IF_CASES_TAC \\ fs []
-  THEN1
-  (fs [adj_stk_bignum_def]
-    \\ fs [eq_eval,wordSemTheory.set_vars_def,alist_insert_def]
+  THEN1 (
+    fs [eq_eval,wordSemTheory.set_vars_def,alist_insert_def]
     \\ fs [dataSemTheory.call_env_def,alist_insert_def,push_env_def,
            dataSemTheory.set_var_def,wordSemTheory.set_vars_def]
     \\ fs [state_rel_thm,lookup_insert,adjust_var_11]
@@ -7216,7 +7212,7 @@ Proof
     \\ reverse conj_tac
     >- fs [labPropsTheory.good_dimindex_def, dimword_def]
     \\ fs [quad_times_div_half_double])
-  \\ fs [adj_stk_bignum_def,stack_consumed_def,OPTION_MAP2_NONE,libTheory.the_def]
+  \\ fs [stack_consumed_def,OPTION_MAP2_NONE,libTheory.the_def]
   \\ rewrite_tac [list_Seq_def]
   \\ fs [dataSemTheory.call_env_def,alist_insert_def,push_env_def,
          dataSemTheory.set_var_def,wordSemTheory.set_vars_def]
@@ -7257,13 +7253,12 @@ Proof
   \\ Cases_on `i1` \\ fs [Smallnum_def]
 QED
 
-(*
+
 Theorem assign_Div:
    op = Div ==> ^assign_thm_goal
 Proof
   rpt strip_tac \\ drule0 (evaluate_GiveUp |> GEN_ALL) \\ rw [] \\ fs []
   \\ `t.termdep <> 0` by fs[]
-  \\ `~s2.safe_for_space` by cheat \\ asm_rewrite_tac [] \\ pop_assum kall_tac
   \\ rpt_drule0 state_rel_cut_IMP
   \\ imp_res_tac get_vars_IMP_LENGTH \\ fs [] \\ rw []
   \\ fs [EVAL ``op_requires_names Div``]
@@ -7300,7 +7295,7 @@ Proof
     \\ `small_int (:α) (&(n1 DIV n2))` by
      (fs [small_int_def,DIV_LT_X]
       \\ rfs [good_dimindex_def,state_rel_thm,dimword_def] \\ rfs [])
-    \\ Cases_on `c.has_div` \\ fs [] THEN1
+   \\ Cases_on `c.has_div` \\ fs [] THEN1
      (fs [list_Seq_def,eq_eval,wordSemTheory.inst_def,insert_shadow]
       \\ once_rewrite_tac [word_exp_set_var_ShiftVar_lemma] \\ fs [eq_eval]
       \\ simp [state_rel_thm,adjust_var_11,
@@ -7314,6 +7309,7 @@ Proof
              dataSemTheory.call_env_def,alist_insert_def,
              push_env_def,dataSemTheory.set_var_def,wordSemTheory.set_vars_def]
       \\ conj_tac THEN1 (rw [] \\ fs [])
+      \\ conj_tac >- rw [option_le_max_right]
       \\ fs [inter_insert_ODD_adjust_set]
       \\ full_simp_tac std_ss [GSYM APPEND_ASSOC]
       \\ match_mp_tac memory_rel_insert
@@ -7341,6 +7337,7 @@ Proof
              FLOOKUP_UPDATE,dataSemTheory.call_env_def,alist_insert_def,
              push_env_def,dataSemTheory.set_var_def,wordSemTheory.set_vars_def]
       \\ conj_tac THEN1 (rw [] \\ fs [])
+      \\ conj_tac >- rw [option_le_max_right]
       \\ fs [inter_insert_ODD_adjust_set]
       \\ full_simp_tac std_ss [GSYM APPEND_ASSOC]
       \\ match_mp_tac memory_rel_insert
@@ -7398,6 +7395,8 @@ Proof
       \\ drule0 (GEN_ALL adjust_var_cut_env_IMP_MEM) \\ fs []
       \\ drule0 (GEN_ALL cut_env_IMP_MEM) \\ fs []
       \\ strip_tac \\ fs [])
+    \\ conj_tac >- cheat
+    \\ conj_tac >- (fs [stack_consumed_def] \\ cheat)
     \\ fs [inter_insert_ODD_adjust_set]
     \\ full_simp_tac std_ss [GSYM APPEND_ASSOC]
     \\ match_mp_tac memory_rel_insert
@@ -7421,18 +7420,50 @@ Proof
     \\ fs [domain_lookup,lookup_inter_alt]
     \\ drule0 env_to_list_lookup_equiv
     \\ fs [lookup_fromAList] \\ strip_tac \\ fs [] \\ fs [lookup_inter_alt])
-  \\ pop_assum kall_tac
+  (* these were lost through rewriting at the start of the proof *)
+  \\ `get_vars [a1;a2] x.locals = SOME [(Number i1); (Number i2)]` by fs [get_vars_def]
+  \\ `get_vars (MAP adjust_var [a1;a2]) t = SOME [(Word w1); (Word w2)]` by (
+     fs [wordSemTheory.get_vars_def, wordSemTheory.get_var_def] \\ every_case_tac \\ fs [])
+  \\ qpat_x_assum `state_rel c l1 l2 x t [] locs` (fn th => NTAC 2 (mp_tac th))
+  \\ strip_tac
+  \\ simp_tac std_ss [Once state_rel_thm] \\ strip_tac \\ fs [] \\ eval_tac
+  \\ full_simp_tac std_ss [GSYM APPEND_ASSOC]
+  \\ rpt_drule0 (memory_rel_get_vars_IMP |> GEN_ALL)
+  \\ strip_tac \\ fs []
+  \\ `~(small_enough_int i1 ∧ small_enough_int i2 ∧ 0 <= i1 /\ 0 <= i2 /\
+        small_enough_int (i1 / i2))` by (
+    CCONTR_TAC \\ fs []
+    \\ `~word_bit 0 w1` by (spose_not_then strip_assume_tac
+    \\ imp_res_tac memory_rel_small_enough_int)
+    \\ fs []
+    \\ drule memory_rel_swap
+    \\ strip_tac
+    \\ `~word_bit 0 w2` by (spose_not_then strip_assume_tac
+    \\ imp_res_tac memory_rel_small_enough_int)
+    \\ fs []
+    \\ first_x_assum (mp_then (Pos last) mp_tac (GEN_ALL memory_rel_Number_IMP))
+    \\ first_x_assum (mp_then (Pos last) mp_tac (GEN_ALL memory_rel_Number_IMP))
+    \\ rpt strip_tac \\ rfs []
+    \\ imp_res_tac NONNEG_INT
+    \\ fs [word_bit_or, word_bit_lsr_dimindex_1, small_int_def, Smallnum_def]
+    \\ rveq
+    \\ fs [word_msb_n2w_numeric, backend_commonTheory.small_enough_int_def,
+       INT_MIN_def, good_dimindex_def, dimword_def] \\ rveq \\ fs [])
+  \\ fs [stack_consumed_def,OPTION_MAP2_NONE,libTheory.the_def]
   \\ fs [list_Seq_def]
   \\ once_rewrite_tac [wordSemTheory.evaluate_def] \\ fs []
   \\ fs [dataSemTheory.call_env_def,alist_insert_def,push_env_def,
          dataSemTheory.set_var_def,wordSemTheory.set_vars_def]
   \\ imp_res_tac cut_state_opt_IMP_ffi \\ fs []
+  \\ rewrite_tac [GSYM state_rel_upd_safe_pkheap]
   \\ match_mp_tac (eval_Call_Div |> REWRITE_RULE [list_Seq_def])
   \\ fs [get_vars_SOME_IFF_data,insert_shadow]
   \\ fs [GSYM wordSemTheory.set_var_def]
   \\ fs [wordSemTheory.set_var_def,state_rel_insert_1]
 QED
 
+
+(*
 Theorem assign_Mod:
    op = Mod ==> ^assign_thm_goal
 Proof
